Label inductive cases

Optimizations/DSL/CodeGenAlt.thy
@@ -155,8 +155,11 @@ lemma fresh_var_head:
   using assms
   by (simp add: Literal.rep_eq fresh_literal.rep_eq fresh_string_preserves_head fresh_var_def)
 
+definition starts_with :: "VarName \<Rightarrow> char \<Rightarrow> bool" where
+  "starts_with v c = (hd (String.explode v) = c)"
+
 definition safe_prefix :: "VarName \<Rightarrow> bool" where
-  "safe_prefix v = (hd (String.explode v) \<noteq> CHR ''X'')"
+  "safe_prefix v = (\<not>(starts_with v CHR ''X''))"
 
 fun valid_pattern :: "IRExpr \<Rightarrow> bool" where
   "valid_pattern (VariableExpr vn s) = safe_prefix vn" |
@@ -171,7 +174,7 @@ fun valid_pattern :: "IRExpr \<Rightarrow> bool" where
 lemma fresh_var_prefix:
   assumes "safe_prefix s"
   shows "fresh_var \<Sigma> \<noteq> s"
-  using assms unfolding safe_prefix_def
+  using assms unfolding safe_prefix_def starts_with_def
   by (metis Fresh_String.Fresh Literal.rep_eq add_Suc_right fresh_literal.rep_eq fresh_string_preserves_head fresh_var_def list.sel(1) list.size(4) zero_less_Suc)
 
 lemma prefix_preserves_freshness:
@@ -194,22 +197,32 @@ lemma freshness:
 
 inductive lower :: "IRExpr \<Rightarrow> VarName set \<Rightarrow> MATCH \<Rightarrow> VarName \<Rightarrow> VarName set \<Rightarrow> bool"
   ("[_, _] \<leadsto> [_, _, _]" 70) where
+  VariableUnseen:
   "vn \<notin> \<Sigma> \<Longrightarrow> [VariableExpr vn s, \<Sigma>] \<leadsto> [noop vn, vn, \<Sigma> \<union> {vn}]" |
-  "vn \<in> \<Sigma> \<and> v' = fresh_var \<Sigma> \<Longrightarrow> [VariableExpr vn s, \<Sigma>] \<leadsto> [v' == vn, v', \<Sigma> \<union> {v'}]" |
+  VariableSeen:
+  "\<lbrakk>vn \<in> \<Sigma>; v' = fresh_var \<Sigma>\<rbrakk> \<Longrightarrow> [VariableExpr vn s, \<Sigma>] \<leadsto> [v' == vn, v', \<Sigma> \<union> {v'}]" |
+  ConstantPattern:
   "v' = fresh_var \<Sigma> \<Longrightarrow> [ConstantExpr c, \<Sigma>] \<leadsto> [match v' (ConstantPattern c), v', \<Sigma> \<union> {v'}]" |
+  UnaryPattern:
   "\<lbrakk>[x, \<Sigma>] \<leadsto> [x\<^sub>m, x\<^sub>v, \<Sigma>\<^sub>x];
     v' = fresh_var \<Sigma>\<^sub>x\<rbrakk>
   \<Longrightarrow> [UnaryExpr op x, \<Sigma>] \<leadsto> [match v' (UnaryPattern op x\<^sub>v) && x\<^sub>m, v', \<Sigma>\<^sub>x \<union> {v'}]" |
+  BinaryPattern:
   "\<lbrakk>[x, \<Sigma>] \<leadsto> [x\<^sub>m, x\<^sub>v, \<Sigma>\<^sub>x]; [y, \<Sigma>\<^sub>x] \<leadsto> [y\<^sub>m, y\<^sub>v, \<Sigma>\<^sub>y];
     v' = fresh_var \<Sigma>\<^sub>y\<rbrakk>
   \<Longrightarrow> [BinaryExpr op x y, \<Sigma>] \<leadsto> [match v' (BinaryPattern op x\<^sub>v y\<^sub>v) && x\<^sub>m && y\<^sub>m, v', \<Sigma>\<^sub>y \<union> {v'}]" |
+  ConditionalPattern:
   "\<lbrakk>[c, \<Sigma>] \<leadsto> [c\<^sub>m, c\<^sub>v, \<Sigma>\<^sub>c]; [t, \<Sigma>\<^sub>c] \<leadsto> [t\<^sub>m, t\<^sub>v, \<Sigma>\<^sub>t];
     [f, \<Sigma>\<^sub>t] \<leadsto> [f\<^sub>m, f\<^sub>v, \<Sigma>\<^sub>f]; v' = fresh_var \<Sigma>\<^sub>f\<rbrakk>
   \<Longrightarrow> [ConditionalExpr c t f, \<Sigma>] \<leadsto> [match v' (ConditionalPattern c\<^sub>v t\<^sub>v f\<^sub>v) && c\<^sub>m && t\<^sub>m && f\<^sub>m, v', \<Sigma>\<^sub>f \<union> {v'}]" |
 
+  ConstantVariableUnseen:
   "vn \<notin> \<Sigma> \<Longrightarrow> [ConstantVar vn, \<Sigma>] \<leadsto> [noop vn, vn, \<Sigma> \<union> {vn}]" | \<comment> \<open>Note that constant variables are also not properly handled currently.\<close>
+  ConstantVariableSeen:
   "vn \<in> \<Sigma> \<and> v' = fresh_var \<Sigma> \<Longrightarrow> [ConstantVar vn, \<Sigma>] \<leadsto> [v' == vn, v', \<Sigma> \<union> {v'}]" |
+  ParameterPattern:
   "v' = fresh_var \<Sigma> \<Longrightarrow> [ParameterExpr nid s, \<Sigma>] \<leadsto> [match v' (ParameterPattern nid), v', \<Sigma> \<union> {v'}]" |
+  LeafPattern:
   "v' = fresh_var \<Sigma> \<Longrightarrow> [LeafExpr nid s, \<Sigma>] \<leadsto> [match v' (LeafPattern nid), v', \<Sigma> \<union> {v'}]"
 
 code_pred (modes: i \<Rightarrow> i \<Rightarrow> o \<Rightarrow> o \<Rightarrow> o \<Rightarrow> bool as lowerC) lower .
@@ -274,58 +287,59 @@ lemma lower_sigma_update2:
   assumes "[e, \<Sigma>] \<leadsto> [m, v, \<Sigma>']"
   shows "\<Sigma> \<inter> ({v} \<union> use_vars m \<union> def_vars m) = {}"
   using assms(2,1) proof (induction rule: lower.induct)
-  case (1 vn \<Sigma> s)
+  case (VariableUnseen vn \<Sigma> s)
   then show ?case by simp
 next
-  case (2 vn \<Sigma> v' s)
+  case (VariableSeen vn \<Sigma> v' s)
   then show ?case
     by (simp add: freshness)
 next
-  case (3 v' \<Sigma> c)
+  case (ConstantPattern v' \<Sigma> c)
   then show ?case
     by (simp add: freshness)
 next
-  case (4 x \<Sigma> x\<^sub>m x\<^sub>v \<Sigma>\<^sub>x v' op)
+  case (UnaryPattern x \<Sigma> x\<^sub>m x\<^sub>v \<Sigma>\<^sub>x v' op)
   have ih: "\<Sigma> \<inter> ({x\<^sub>v} \<union> use_vars x\<^sub>m \<union> def_vars x\<^sub>m) = {}"
-    using "4.IH" "4.prems" by presburger
+    using UnaryPattern by presburger
   have seq: "({v'} \<union> use_vars (match v' (UnaryPattern op x\<^sub>v) && x\<^sub>m) \<union> def_vars (match v' (UnaryPattern op x\<^sub>v) && x\<^sub>m)) 
     = {v'} \<union> use_vars x\<^sub>m \<union> {x\<^sub>v} \<union> def_vars x\<^sub>m"
     by simp
   then show ?case
-    by (metis "4.IH" "4.hyps"(1) "4.hyps"(2) "4.prems" Int_insert_right UnCI Un_assoc Un_commute freshness insert_is_Un lower_finite lower_sigma_update)
+    by (metis UnaryPattern Int_insert_right UnCI Un_assoc Un_commute freshness insert_is_Un lower_finite lower_sigma_update)
 next
-  case (5 x \<Sigma> x\<^sub>m x\<^sub>v \<Sigma>\<^sub>x y y\<^sub>m y\<^sub>v \<Sigma>\<^sub>y v' op)
+  case (BinaryPattern x \<Sigma> x\<^sub>m x\<^sub>v \<Sigma>\<^sub>x y y\<^sub>m y\<^sub>v \<Sigma>\<^sub>y v' op)
   have ihx: "\<Sigma> \<inter> ({x\<^sub>v} \<union> use_vars x\<^sub>m \<union> def_vars x\<^sub>m) = {}"
-    using "5.IH"(1) "5.prems" by blast
+    using BinaryPattern by blast
   have ihy: "\<Sigma>\<^sub>x \<inter> ({y\<^sub>v} \<union> use_vars y\<^sub>m \<union> def_vars y\<^sub>m) = {}"
-    using "5.IH"(2) "5.hyps"(1) "5.prems" lower_finite by presburger
+    using BinaryPattern lower_finite by presburger
   then have ihy': "(\<Sigma> \<union> {x\<^sub>v} \<union> def_vars x\<^sub>m) \<inter> ({y\<^sub>v} \<union> use_vars y\<^sub>m \<union> def_vars y\<^sub>m) = {}"
-    using "5.hyps"(1) lower_sigma_update by presburger
+    using BinaryPattern lower_sigma_update by presburger
   have seq: "({v'} \<union> use_vars (match v' (BinaryPattern op x\<^sub>v y\<^sub>v) && x\<^sub>m && y\<^sub>m) \<union> def_vars (match v' (BinaryPattern op x\<^sub>v y\<^sub>v) && x\<^sub>m && y\<^sub>m))
     = {v'} \<union> use_vars x\<^sub>m \<union> use_vars y\<^sub>m \<union> {x\<^sub>v, y\<^sub>v} \<union> def_vars x\<^sub>m \<union> def_vars y\<^sub>m"
     by force
   then show ?case using seq ihx ihy' apply simp
-    by (smt (verit) "5.hyps"(1) "5.hyps"(2) "5.hyps"(3) "5.prems" Un_iff disjoint_iff_not_equal freshness lower_finite lower_sigma_update)
+    by (smt (verit) BinaryPattern.hyps(1) BinaryPattern.hyps(2) BinaryPattern.hyps(3) BinaryPattern.prems Un_iff disjoint_iff_not_equal freshness lower_finite lower_sigma_update)
 next
-  case (6 c \<Sigma> c\<^sub>m c\<^sub>v \<Sigma>\<^sub>c t t\<^sub>m t\<^sub>v \<Sigma>\<^sub>t f f\<^sub>m f\<^sub>v \<Sigma>\<^sub>f v')
+  case (ConditionalPattern c \<Sigma> c\<^sub>m c\<^sub>v \<Sigma>\<^sub>c t t\<^sub>m t\<^sub>v \<Sigma>\<^sub>t f f\<^sub>m f\<^sub>v \<Sigma>\<^sub>f v')
   have ihc: "\<Sigma> \<inter> ({c\<^sub>v} \<union> use_vars c\<^sub>m \<union> def_vars c\<^sub>m) = {}"
-    using "6.IH"(1) "6.prems" by auto
+    using ConditionalPattern by auto
   have iht: "\<Sigma>\<^sub>c \<inter> ({t\<^sub>v} \<union> use_vars t\<^sub>m \<union> def_vars t\<^sub>m) = {}"
-    using "6.IH"(2) "6.hyps"(1) "6.prems" lower_finite by blast
+    using ConditionalPattern lower_finite by blast
   have ihf: "\<Sigma>\<^sub>t \<inter> ({f\<^sub>v} \<union> use_vars f\<^sub>m \<union> def_vars f\<^sub>m) = {}"
-    by (meson "6.IH"(3) "6.hyps"(1) "6.hyps"(2) "6.prems" lower_finite)
+    by (meson ConditionalPattern lower_finite)
   have iht': "(\<Sigma> \<union> {c\<^sub>v} \<union> def_vars c\<^sub>m) \<inter> ({t\<^sub>v} \<union> use_vars t\<^sub>m \<union> def_vars t\<^sub>m) = {}"
-    using "6.hyps"(1) iht lower_sigma_update by presburger
+    using ConditionalPattern iht lower_sigma_update by presburger
   then have ihf': "(\<Sigma> \<union> {c\<^sub>v} \<union> def_vars c\<^sub>m \<union> {t\<^sub>v} \<union> def_vars t\<^sub>m) \<inter> ({f\<^sub>v} \<union> use_vars f\<^sub>m \<union> def_vars f\<^sub>m) = {}"
-    using "6.hyps"(1) "6.hyps"(2) ihf lower_sigma_update by presburger
+    using ConditionalPattern ihf lower_sigma_update by presburger
   have seq: "({v'} \<union> use_vars (match v' (ConditionalPattern c\<^sub>v t\<^sub>v f\<^sub>v) && c\<^sub>m && t\<^sub>m && f\<^sub>m) \<union> def_vars (match v' (ConditionalPattern c\<^sub>v t\<^sub>v f\<^sub>v) && c\<^sub>m && t\<^sub>m && f\<^sub>m))
     = {v'} \<union> use_vars c\<^sub>m \<union> use_vars t\<^sub>m \<union> use_vars f\<^sub>m \<union> {c\<^sub>v, t\<^sub>v, f\<^sub>v} \<union> def_vars c\<^sub>m \<union> def_vars t\<^sub>m \<union> def_vars f\<^sub>m"
     by (simp add: Un_assoc)
   then show ?case apply auto
     using ihc apply auto[1] 
     using iht' apply auto[1] 
-    using ihf' apply force 
-    apply (metis "6.hyps"(1) "6.hyps"(2) "6.hyps"(3) "6.hyps"(4) "6.prems" UnI1 freshness lower_finite lower_sigma_update) 
+    using ihf' apply force
+    using UnI1 freshness lower_finite lower_sigma_update
+    apply (metis ConditionalPattern.hyps(1,2,3,4) ConditionalPattern.prems)
     apply (metis Un_iff disjoint_iff ihc) 
     using iht' mk_disjoint_insert apply fastforce 
     using ihf' mk_disjoint_insert apply fastforce 
@@ -333,19 +347,19 @@ next
     using iht' mk_disjoint_insert apply fastforce
     using ihf' mk_disjoint_insert by fastforce
 next
-  case (7 vn \<Sigma>)
+  case (ConstantVariableUnseen vn \<Sigma>)
   then show ?case
     by simp
 next
-  case (8 vn \<Sigma> v')
+  case (ConstantVariableSeen vn \<Sigma> v')
   then show ?case
     by (simp add: freshness)
 next
-  case (9 v' \<Sigma> nid s)
+  case (ParameterPattern v' \<Sigma> nid s)
   then show ?case
     by (simp add: freshness)
 next
-  case (10 v' \<Sigma> nid s)
+  case (LeafPattern v' \<Sigma> nid s)
   then show ?case
     by (simp add: freshness)
 qed 
@@ -357,78 +371,78 @@ lemma lower_valid_matches:
   shows "valid_match m"
   using assms(3,2,1)
 proof (induction rule: lower.induct)
-  case (1 vn \<Sigma> s)
+  case (VariableUnseen vn \<Sigma> s)
   then show ?case by simp
 next
-  case (2 vn \<Sigma> v' s)
+  case (VariableSeen vn \<Sigma> v' s)
   then show ?case by simp
 next
-  case (3 v' \<Sigma> c)
+  case (ConstantPattern v' \<Sigma> c)
   then show ?case by simp
 next
-  case (4 x \<Sigma> x\<^sub>m x\<^sub>v \<Sigma>\<^sub>x v' op)
+  case (UnaryPattern x \<Sigma> x\<^sub>m x\<^sub>v \<Sigma>\<^sub>x v' op)
   have "fresh_var \<Sigma>\<^sub>x \<noteq> x\<^sub>v"
-    using lower_sigma_update 4 freshness
+    using lower_sigma_update UnaryPattern freshness
     by (metis UnCI insertCI lower_finite)
   have "fresh_var \<Sigma>\<^sub>x \<noteq> x\<^sub>v \<and> fresh_var \<Sigma>\<^sub>x \<notin> def_vars x\<^sub>m"
-    by (metis "4.hyps"(1) "4.prems"(2) UnCI \<open>fresh_var \<Sigma>\<^sub>x \<noteq> x\<^sub>v\<close> freshness lower_finite lower_sigma_update)
-  then show ?case using 4 by simp
+    by (metis "UnaryPattern.hyps"(1) "UnaryPattern.prems"(2) UnCI \<open>fresh_var \<Sigma>\<^sub>x \<noteq> x\<^sub>v\<close> freshness lower_finite lower_sigma_update)
+  then show ?case using UnaryPattern by simp
 next
-  case (5 x \<Sigma> x\<^sub>m x\<^sub>v \<Sigma>\<^sub>x y y\<^sub>m y\<^sub>v \<Sigma>\<^sub>y v' op)
+  case (BinaryPattern x \<Sigma> x\<^sub>m x\<^sub>v \<Sigma>\<^sub>x y y\<^sub>m y\<^sub>v \<Sigma>\<^sub>y v' op)
   have vmx: "valid_match x\<^sub>m"
-    using "5.IH"(1) "5.prems"(1) "5.prems"(2) by fastforce
+    using BinaryPattern by fastforce
   have vmy: "valid_match y\<^sub>m"
-    using "5.IH"(2) "5.hyps"(1) "5.prems" lower_finite
+    using BinaryPattern lower_finite
     by (metis UnCI \<L>.simps(5))
-  have "fresh_var \<Sigma>\<^sub>y \<noteq> x\<^sub>v" using 5
+  have "fresh_var \<Sigma>\<^sub>y \<noteq> x\<^sub>v" using BinaryPattern
     by (metis UnCI freshness insertCI lower_finite lower_sigma_update)
-  also have "fresh_var \<Sigma>\<^sub>y \<noteq> y\<^sub>v" using 5
+  also have "fresh_var \<Sigma>\<^sub>y \<noteq> y\<^sub>v" using BinaryPattern
     by (metis UnCI freshness insertCI lower_finite lower_sigma_update)
-  moreover have "use_vars x\<^sub>m \<inter> def_vars y\<^sub>m = {}" using 5 lower_sigma_update2
+  moreover have "use_vars x\<^sub>m \<inter> def_vars y\<^sub>m = {}" using BinaryPattern lower_sigma_update2
     by (metis UnCI disjoint_iff_not_equal lower_finite lower_sigma_update1)
-  moreover have "x\<^sub>v \<noteq> y\<^sub>v" using 5
+  moreover have "x\<^sub>v \<noteq> y\<^sub>v" using BinaryPattern
     by (metis Un_commute Un_insert_right disjoint_insert(2) insertI1 lower_finite lower_sigma_update lower_sigma_update2)
   ultimately have "fresh_var \<Sigma>\<^sub>y \<noteq> x\<^sub>v \<and> fresh_var \<Sigma>\<^sub>y \<noteq> y\<^sub>v \<and> x\<^sub>v \<noteq> y\<^sub>v \<and> use_vars x\<^sub>m \<inter> def_vars y\<^sub>m = {} \<and> fresh_var \<Sigma>\<^sub>y \<notin> def_vars x\<^sub>m \<and> fresh_var \<Sigma>\<^sub>y \<notin> def_vars y\<^sub>m"
-    by (metis "5.hyps"(1) "5.hyps"(2) "5.prems"(2) UnCI freshness lower_finite lower_sigma_update)
+    by (metis BinaryPattern.hyps(1,2) BinaryPattern.prems(2) UnCI freshness lower_finite lower_sigma_update)
   then show ?case
-    by (simp add: "5.hyps"(3) vmx vmy)
+    by (simp add: BinaryPattern.hyps(3) vmx vmy)
 next
-  case (6 c \<Sigma> c\<^sub>m c\<^sub>v \<Sigma>\<^sub>c t t\<^sub>m t\<^sub>v \<Sigma>\<^sub>t f f\<^sub>m f\<^sub>v \<Sigma>\<^sub>f v')
+  case (ConditionalPattern c \<Sigma> c\<^sub>m c\<^sub>v \<Sigma>\<^sub>c t t\<^sub>m t\<^sub>v \<Sigma>\<^sub>t f f\<^sub>m f\<^sub>v \<Sigma>\<^sub>f v')
   have vmc: "valid_match c\<^sub>m"
-    using "6.IH"(1) "6.prems"(1) "6.prems"(2) by force
+    using ConditionalPattern by force
   have vmt: "valid_match t\<^sub>m"
-    using "6.IH"(2) "6.hyps"(1) "6.prems"(1) "6.prems"(2) lower_finite by auto
+    using ConditionalPattern lower_finite by auto
   have vmf: "valid_match f\<^sub>m"
-    by (metis "6.IH"(3) "6.hyps"(1) "6.hyps"(2) "6.prems"(1) "6.prems"(2) UnI2 \<L>.simps(6) lower_finite)
+    by (metis ConditionalPattern UnI2 \<L>.simps(6) lower_finite)
   have v'ne: "v' \<noteq> c\<^sub>v \<and> v' \<noteq> t\<^sub>v \<and> v' \<noteq> f\<^sub>v"
-    by (smt (verit) "6.hyps"(1) "6.hyps"(2) "6.hyps"(3) "6.hyps"(4) "6.prems"(2) Un_insert_left Un_insert_right freshness insert_iff lower_finite lower_sigma_update)
+    by (smt (verit) ConditionalPattern Un_insert_left Un_insert_right freshness insert_iff lower_finite lower_sigma_update)
   have dij: "c\<^sub>v \<noteq> t\<^sub>v \<and> c\<^sub>v \<noteq> f\<^sub>v \<and> t\<^sub>v \<noteq> f\<^sub>v"
-    by (metis "6.hyps"(1) "6.hyps"(2) "6.hyps"(3) "6.prems"(2) UnCI Un_insert_left disjoint_insert(2) insertCI lower_finite lower_sigma_update1 lower_sigma_update2)
+    by (metis ConditionalPattern UnCI Un_insert_left disjoint_insert(2) insertCI lower_finite lower_sigma_update1 lower_sigma_update2)
   have cd: "use_vars c\<^sub>m \<inter> (def_vars t\<^sub>m \<union> def_vars f\<^sub>m) = {}"
-    using 6 lower_sigma_update2
+    using ConditionalPattern lower_sigma_update2
     by (smt (verit, ccfv_threshold) Un_iff disjoint_iff lower_finite lower_sigma_update1)
   have td: "use_vars t\<^sub>m \<inter> def_vars f\<^sub>m = {}"
-    using 6 lower_sigma_update2
+    using ConditionalPattern lower_sigma_update2
     by (smt (verit, ccfv_SIG) UnCI disjoint_iff lower_finite lower_sigma_update1)
   have "v' \<notin> def_vars c\<^sub>m \<and> v' \<notin> def_vars t\<^sub>m \<and> v' \<notin> def_vars f\<^sub>m"
-    using 6
+    using ConditionalPattern
     by (metis UnI1 Un_insert_right freshness insertCI lower_finite lower_sigma_update mk_disjoint_insert)
   then show ?case using vmc vmt vmf v'ne dij cd td
     by simp
 next
-  case (7 vn \<Sigma>)
+  case (ConstantVariableUnseen vn \<Sigma>)
   then show ?case
     by simp
 next
-  case (8 vn v' \<Sigma>)
+  case (ConstantVariableSeen vn v' \<Sigma>)
   then show ?case
     by simp
 next
-  case (9 v' \<Sigma> nid s)
+  case (ParameterPattern v' \<Sigma> nid s)
   then show ?case
     by simp
 next
-  case (10 v' \<Sigma> nid s)
+  case (LeafPattern v' \<Sigma> nid s)
   then show ?case
     by simp
 qed
@@ -438,8 +452,8 @@ subsection \<open>MATCH Matching Semantics\<close>
 
 inductive unify :: "Subst \<Rightarrow> (VarName \<times> IRExpr) list \<Rightarrow> Subst \<Rightarrow> bool" where
   "unify \<sigma> [] \<sigma>" |
-  "v \<in> dom \<sigma> \<and> \<sigma> v = Some e \<and> unify \<sigma> xs \<sigma>' \<Longrightarrow> unify \<sigma> ((v, e) # xs) \<sigma>'" |
-  "v \<notin> dom \<sigma> \<and> unify (\<sigma>(v \<mapsto> e)) xs \<sigma>' \<Longrightarrow> unify \<sigma> ((v, e) # xs) \<sigma>'"
+  "\<lbrakk>v \<in> dom \<sigma>; \<sigma> v = Some e; unify \<sigma> xs \<sigma>'\<rbrakk> \<Longrightarrow> unify \<sigma> ((v, e) # xs) \<sigma>'" |
+  "\<lbrakk>v \<notin> dom \<sigma>; unify (\<sigma>(v \<mapsto> e)) xs \<sigma>'\<rbrakk> \<Longrightarrow> unify \<sigma> ((v, e) # xs) \<sigma>'"
 
 lemma unify_grows:
   assumes "unify \<sigma> xs \<sigma>'"
@@ -461,14 +475,23 @@ lemma unify_update:
   apply simp using unify_grows by fastforce+
 
 inductive eval_match :: "MATCH \<Rightarrow> Subst \<Rightarrow> Subst \<Rightarrow> bool" ("_ \<U> _ = _" 70) where
-  "\<sigma> v = Some (UnaryExpr op xe) \<and> unify \<sigma> [(x, xe)] \<sigma>' \<Longrightarrow> (match v (UnaryPattern op x)) \<U> \<sigma> = \<sigma>'" |
-  "\<sigma> v = Some (BinaryExpr op xe ye) \<and> unify \<sigma> [(x, xe), (y, ye)] \<sigma>' \<Longrightarrow> (match v (BinaryPattern op x y)) \<U> \<sigma> = \<sigma>'" |
-  "\<sigma> v = Some (ConditionalExpr ce te fe) \<and> unify \<sigma> [(c, ce), (t, te), (f, fe)] \<sigma>' \<Longrightarrow> (match v (ConditionalPattern c t f)) \<U> \<sigma> = \<sigma>'" |
+  UnaryPattern:
+  "\<lbrakk>\<sigma> v = Some (UnaryExpr op xe); unify \<sigma> [(x, xe)] \<sigma>'\<rbrakk> \<Longrightarrow> (match v (UnaryPattern op x)) \<U> \<sigma> = \<sigma>'" |
+  BinaryPattern:
+  "\<lbrakk>\<sigma> v = Some (BinaryExpr op xe ye); unify \<sigma> [(x, xe), (y, ye)] \<sigma>'\<rbrakk> \<Longrightarrow> (match v (BinaryPattern op x y)) \<U> \<sigma> = \<sigma>'" |
+  ConditionalPattern:
+  "\<lbrakk>\<sigma> v = Some (ConditionalExpr ce te fe); unify \<sigma> [(c, ce), (t, te), (f, fe)] \<sigma>'\<rbrakk> \<Longrightarrow> (match v (ConditionalPattern c t f)) \<U> \<sigma> = \<sigma>'" |
+  ConstantPattern:
   "\<sigma> v = Some (ConstantExpr c) \<Longrightarrow> (match v (ConstantPattern c)) \<U> \<sigma> = \<sigma>" |
+  ParameterPattern:
   "\<sigma> v = Some (ParameterExpr nid s) \<Longrightarrow> (match v (ParameterPattern nid)) \<U> \<sigma> = \<sigma>" |
+  LeafPattern:
   "\<sigma> v = Some (LeafExpr nid s) \<Longrightarrow> (match v (LeafPattern nid)) \<U> \<sigma> = \<sigma>" |
+  Equality:
   "v\<^sub>1 \<in> dom \<sigma> \<and> v\<^sub>2 \<in> dom \<sigma> \<and> \<sigma> v\<^sub>1 = \<sigma> v\<^sub>2 \<Longrightarrow> (v\<^sub>1 == v\<^sub>2) \<U> \<sigma> = \<sigma>" |
+  AndThen:
   "(m\<^sub>1 \<U> \<sigma> = \<sigma>') \<and> (m\<^sub>2 \<U> \<sigma>' = \<sigma>'') \<Longrightarrow> (m\<^sub>1 && m\<^sub>2) \<U> \<sigma> = \<sigma>''" |
+  Noop:
   "v \<in> dom \<sigma> \<Longrightarrow> noop v \<U> \<sigma> = \<sigma>"
 
 code_pred (modes: i \<Rightarrow> i \<Rightarrow> o \<Rightarrow> bool as eval_matchC) eval_match .
@@ -590,54 +613,54 @@ lemma eval_match_adds_patterns:
   assumes "m \<U> \<sigma> = \<sigma>'"
   shows "\<L> e \<subseteq> dom \<sigma>'"
   using assms proof (induct arbitrary: v \<Sigma>' \<sigma> \<sigma>' rule: lower.induct)
-  case (1 vn \<Sigma> s)
+  case (VariableUnseen vn \<Sigma> s)
   then show ?case
     by (metis \<L>.simps(1) eval_match_noop singletonD subsetI)
 next
-  case (2 vn \<Sigma> v' s)
+  case (VariableSeen vn \<Sigma> v' s)
   then show ?case 
     by (metis \<L>.simps(1) eval_match_equality singletonD subsetI)
 next
-  case (3 v' \<Sigma> c)
+  case (ConstantPattern v' \<Sigma> c)
   then show ?case by simp
 next
-  case (4 x \<Sigma> x\<^sub>m x\<^sub>v \<Sigma>\<^sub>x v' op)
+  case (UnaryPattern x \<Sigma> x\<^sub>m x\<^sub>v \<Sigma>\<^sub>x v' op)
   then show ?case
     by (metis \<L>.simps(4) eval_match_andthen valid_match.simps(4))
 next
-  case (5 x \<Sigma> x\<^sub>m x\<^sub>v \<Sigma>\<^sub>x y y\<^sub>m y\<^sub>v \<Sigma>\<^sub>y v' op)
+  case (BinaryPattern x \<Sigma> x\<^sub>m x\<^sub>v \<Sigma>\<^sub>x y y\<^sub>m y\<^sub>v \<Sigma>\<^sub>y v' op)
   obtain \<sigma>\<^sub>m where \<sigma>\<^sub>m: "match v' (BinaryPattern op x\<^sub>v y\<^sub>v) \<U> \<sigma> = \<sigma>\<^sub>m"
-    by (meson "5.prems" eval_match_andthen)
+    by (meson BinaryPattern.prems eval_match_andthen)
   then obtain \<sigma>\<^sub>x where \<sigma>\<^sub>x: "x\<^sub>m \<U> \<sigma>\<^sub>m = \<sigma>\<^sub>x"
-    by (metis "5.prems"(2) eval_match_andthen eval_match_deterministic)
+    by (metis BinaryPattern.prems(2) eval_match_andthen eval_match_deterministic)
   then obtain \<sigma>\<^sub>y where \<sigma>\<^sub>y: "y\<^sub>m \<U> \<sigma>\<^sub>x = \<sigma>\<^sub>y"
-    by (metis "5.prems"(2) \<open>match v' (BinaryPattern op x\<^sub>v y\<^sub>v) \<U> \<sigma> = \<sigma>\<^sub>m\<close> eval_match_andthen eval_match_deterministic)
+    by (metis BinaryPattern.prems(2) \<open>match v' (BinaryPattern op x\<^sub>v y\<^sub>v) \<U> \<sigma> = \<sigma>\<^sub>m\<close> eval_match_andthen eval_match_deterministic)
   have xs: "\<L> x \<subseteq> dom \<sigma>\<^sub>x"
-    using "5.hyps"(2) \<sigma>\<^sub>x "5.prems"(1) by auto
+    using BinaryPattern.hyps(2) \<sigma>\<^sub>x BinaryPattern.prems(1) by auto
   have ys: "\<L> y \<subseteq> dom \<sigma>\<^sub>y"
-    using "5.hyps"(4) \<sigma>\<^sub>y "5.prems"(1) by auto
+    using BinaryPattern.hyps(4) \<sigma>\<^sub>y BinaryPattern.prems(1) by auto
   have "\<L> (BinaryExpr op x y) = \<L> x \<union> \<L> y"
     by simp
   have "dom \<sigma>\<^sub>x \<union> dom \<sigma>\<^sub>y \<subseteq> dom \<sigma>'"
-    by (metis "5.prems"(1) "5.prems"(2) \<sigma>\<^sub>m \<sigma>\<^sub>x \<sigma>\<^sub>y dual_order.eq_iff eval_match.intros(8) eval_match_deterministic eval_match_subset map_le_implies_dom_le sup_absorb2 valid_match.simps(4))
+    by (metis BinaryPattern.prems(1,2) \<sigma>\<^sub>m \<sigma>\<^sub>x \<sigma>\<^sub>y dual_order.eq_iff eval_match.intros(8) eval_match_deterministic eval_match_subset map_le_implies_dom_le sup_absorb2 valid_match.simps(4))
   then show ?case
     by (metis Un_subset_iff \<open>\<L> (BinaryExpr op x y) = \<L> x \<union> \<L> y\<close> sup.absorb_iff1 xs ys)
 next
-  case (6 c \<Sigma> c\<^sub>m c\<^sub>v \<Sigma>\<^sub>c t t\<^sub>m t\<^sub>v \<Sigma>\<^sub>t f f\<^sub>m f\<^sub>v \<Sigma>\<^sub>f v')
+  case (ConditionalPattern c \<Sigma> c\<^sub>m c\<^sub>v \<Sigma>\<^sub>c t t\<^sub>m t\<^sub>v \<Sigma>\<^sub>t f f\<^sub>m f\<^sub>v \<Sigma>\<^sub>f v')
   then show ?case sorry
 next
-  case (7 vn \<Sigma>)
+  case (ConstantVariableUnseen vn \<Sigma>)
   then show ?case
     by (metis \<L>.simps(2) eval_match_noop singletonD subsetI)
 next
-  case (8 vn \<Sigma> v')
+  case (ConstantVariableSeen vn \<Sigma> v')
   then show ?case
     by (metis \<L>.simps(2) eval_match_equality singletonD subsetI)
 next
-  case (9 v' \<Sigma> nid s)
+  case (ParameterPattern v' \<Sigma> nid s)
   then show ?case by simp
 next
-  case (10 v' \<Sigma> nid s)
+  case (LeafPattern v' \<Sigma> nid s)
   then show ?case by simp
 qed
 
@@ -668,96 +691,96 @@ theorem lower_sound:
   assumes "m \<U> \<sigma>(v \<mapsto> e') = \<sigma>'"
   shows "match_tree e e' = Some (\<sigma>'|`(\<L> e))"
   using assms(3,2,1,4) proof (induct arbitrary: \<sigma> e' \<sigma>' rule: lower.induct)
-  case (1 vn \<Sigma> s)
+  case (VariableUnseen vn \<Sigma> s)
   have "\<sigma>' = \<sigma>(vn \<mapsto> e')"
-    using "1.prems"
+    using VariableUnseen.prems
     by (meson eval_match_noop)
   then have "(\<sigma>' |` \<L> (VariableExpr vn s)) = (\<sigma> |` \<L> (VariableExpr vn s))(vn \<mapsto> e')"
     by simp
   then show ?case
     by force
 next
-  case (2 vn \<Sigma> v' s)
+  case (VariableSeen vn \<Sigma> v' s)
   have "v' \<noteq> vn"
-    using "2.hyps" "2.prems"(2) valid_pattern_preserves_freshness by fastforce
+    using VariableSeen.hyps VariableSeen.prems(2) valid_pattern_preserves_freshness by fastforce
   also have "\<sigma>' = \<sigma>(v' \<mapsto> e')"
-    using "2.prems"(3) calculation(1) 
+    using VariableSeen.prems(3) calculation(1) 
     using eval_match.simps by blast
   ultimately show ?case
-    using "2.prems"(3) eval_match_equality by fastforce
+    using VariableSeen.prems(3) eval_match_equality by fastforce
 next
-  case (3 v' \<Sigma> c)
+  case (ConstantPattern v' \<Sigma> c)
   have "e' = ConstantExpr c"
-    by (meson "3.prems"(3) eval_match_ConstantExpr map_upd_Some_unfold)
+    by (meson ConstantPattern.prems(3) eval_match_ConstantExpr map_upd_Some_unfold)
   then show ?case
     by simp
 next
-  case (4 x \<Sigma> x\<^sub>m x\<^sub>v \<Sigma>\<^sub>x v' op)
+  case (UnaryPattern x \<Sigma> x\<^sub>m x\<^sub>v \<Sigma>\<^sub>x v' op)
   obtain \<sigma>\<^sub>m where m1: "match v' (UnaryPattern op x\<^sub>v) \<U> \<sigma>(v' \<mapsto> e') = \<sigma>\<^sub>m"
-    by (meson "4.prems"(3) eval_match_andthen)
-  then obtain e\<^sub>x where  e': "e' = UnaryExpr op e\<^sub>x" using 4
+    by (meson UnaryPattern.prems(3) eval_match_andthen)
+  then obtain e\<^sub>x where  e': "e' = UnaryExpr op e\<^sub>x" using UnaryPattern
     by (meson eval_match_UnaryPattern map_upd_Some_unfold)
   then have "match_tree x e\<^sub>x = Some (\<sigma>' |` \<L> x)"
   proof -
     have u1: "unify (\<sigma>(v' \<mapsto> e')) [(x\<^sub>v, e\<^sub>x)] \<sigma>\<^sub>m" 
-      using 4 e'
+      using UnaryPattern e'
       by (metis IRExpr.sel(2) m1 eval_match_UnaryPattern fun_upd_same option.sel)
     have "x\<^sub>m \<U> \<sigma>\<^sub>m = \<sigma>'"
-      by (metis "4.prems"(3) m1 eval_match_andthen eval_match_deterministic)
+      by (metis UnaryPattern.prems(3) m1 eval_match_andthen eval_match_deterministic)
     then obtain \<sigma>\<^sub>x where xm: "x\<^sub>m \<U> \<sigma>\<^sub>x(x\<^sub>v \<mapsto> e\<^sub>x) = \<sigma>'"
       using u1 unify_partition
       by (meson list.set_intros(1) map_le_refl)
     then show ?thesis
-      using 4 by fastforce
+      using UnaryPattern by fastforce
   qed
   then show ?case
     using e' by auto
 next
-  case (5 x \<Sigma> x\<^sub>m x\<^sub>v \<Sigma>\<^sub>x y y\<^sub>m y\<^sub>v \<Sigma>\<^sub>y v' op)
+  case (BinaryPattern x \<Sigma> x\<^sub>m x\<^sub>v \<Sigma>\<^sub>x y y\<^sub>m y\<^sub>v \<Sigma>\<^sub>y v' op)
   obtain \<sigma>\<^sub>m where s1: "match v' (BinaryPattern op x\<^sub>v y\<^sub>v) \<U> \<sigma>(v' \<mapsto> e') = \<sigma>\<^sub>m"
-    by (meson "5.prems"(3) eval_match_andthen)
+    by (meson BinaryPattern.prems(3) eval_match_andthen)
   then obtain e\<^sub>x e\<^sub>y where e': "e' = BinaryExpr op e\<^sub>x e\<^sub>y"
     by (meson eval_match_BinaryPattern map_upd_Some_unfold)
   have u1: "unify (\<sigma>(v' \<mapsto> e')) [(x\<^sub>v, e\<^sub>x), (y\<^sub>v, e\<^sub>y)] \<sigma>\<^sub>m"
       using e' IRExpr.inject(2) s1 eval_match_BinaryPattern by fastforce
   then obtain \<sigma>\<^sub>x where m1: "x\<^sub>m \<U> \<sigma>\<^sub>m = \<sigma>\<^sub>x"
-    by (metis "5.prems"(3) eval_match_andthen eval_match_deterministic s1)
+    by (metis BinaryPattern.prems(3) eval_match_andthen eval_match_deterministic s1)
   then have mx: "\<sigma>\<^sub>m \<subseteq>\<^sub>m \<sigma>\<^sub>x"
-    using "5.prems"(2) eval_match_subset m1 
-    by (metis "5.hyps"(1) "5.prems"(1) lower_valid_matches valid_pattern.simps(5) valid_pattern_preserves_freshness)
+    using BinaryPattern.prems(2) eval_match_subset m1 
+    by (metis BinaryPattern.hyps(1) BinaryPattern.prems(1) lower_valid_matches valid_pattern.simps(5) valid_pattern_preserves_freshness)
   then have mt1: "match_tree x e\<^sub>x = Some (\<sigma>\<^sub>x |` \<L> x)"
   proof -
     obtain \<sigma>\<^sub>x' where xm: "x\<^sub>m \<U> \<sigma>\<^sub>x'(x\<^sub>v \<mapsto> e\<^sub>x) = \<sigma>\<^sub>x"
       using m1 u1 unify_partition
       by (meson list.set_intros(1) map_le_refl)
     then show ?thesis
-      using 5 by fastforce
+      using BinaryPattern by fastforce
   qed
   then have mt2: "match_tree y e\<^sub>y = Some (\<sigma>' |` \<L> y)"
   proof -
     have m2: "y\<^sub>m \<U> \<sigma>\<^sub>x = \<sigma>'"
-      by (metis "5.prems"(3) eval_match_andthen eval_match_deterministic m1 s1)
+      by (metis BinaryPattern.prems(3) eval_match_andthen eval_match_deterministic m1 s1)
     then have "\<sigma>\<^sub>m \<subseteq>\<^sub>m \<sigma>\<^sub>x"
-      using "5.prems"(3) eval_match_subset m1
+      using BinaryPattern.prems(3) eval_match_subset m1
       using mx by fastforce
     then obtain \<sigma>\<^sub>y' where ym: "y\<^sub>m \<U> \<sigma>\<^sub>y'(y\<^sub>v \<mapsto> e\<^sub>y) = \<sigma>'"
       using m1 u1 unify_partition
       by (metis list.set_intros(1) m2 unify_unempty)
     then show ?thesis
-      using 5 
+      using BinaryPattern
       using lower_finite valid_pattern.simps(5) by blast
   qed
   have comp: "compatible \<sigma>\<^sub>x \<sigma>'" using mx
     using  CodeGenAlt.compatible.elims(3) eval_match_andthen eval_match_deterministic eval_match_subset m1 map_le_def s1 valid_match.simps(4)
-    by (metis "5.hyps"(1) "5.hyps"(3) "5.prems"(1) "5.prems"(2) "5.prems"(3) lower_finite lower_valid_matches valid_pattern.simps(5) valid_pattern_preserves_freshness)
+    by (metis BinaryPattern.hyps(1,3) BinaryPattern.prems(1,2,3) lower_finite lower_valid_matches valid_pattern.simps(5) valid_pattern_preserves_freshness)
   then have comp': "compatible (\<sigma>\<^sub>x |` \<L> x) (\<sigma>' |` \<L> y)"
     by (metis (full_types) CodeGenAlt.compatible.elims(2) CodeGenAlt.compatible.elims(3) domIff restrict_in restrict_out)
   have "\<sigma>\<^sub>x ++ \<sigma>' = \<sigma>'"
     using mx
-    by (metis "5.hyps"(1) "5.hyps"(3) "5.prems"(1) "5.prems"(2) "5.prems"(3) eval_match_andthen eval_match_deterministic eval_match_subset lower_finite lower_valid_matches m1 map_add_subsumed1 s1 valid_pattern.simps(5) valid_pattern_preserves_freshness)
+    by (metis BinaryPattern.hyps(1,3) BinaryPattern.prems(1,2,3) eval_match_andthen eval_match_deterministic eval_match_subset lower_finite lower_valid_matches m1 map_add_subsumed1 s1 valid_pattern.simps(5) valid_pattern_preserves_freshness)
   have "(dom \<sigma>' - dom \<sigma>\<^sub>x) \<inter> \<L> x = {}" \<comment> \<open>Ian: This is the troublesome case\<close>
     using eval_match_adds_patterns
-    by (metis "5.hyps"(1) "5.prems"(1) "5.prems"(2) DiffD2 disjoint_iff lower_valid_matches m1 subset_eq valid_pattern.simps(5) valid_pattern_preserves_freshness)
+    by (metis BinaryPattern.hyps(1) BinaryPattern.prems(1,2) DiffD2 disjoint_iff lower_valid_matches m1 subset_eq valid_pattern.simps(5) valid_pattern_preserves_freshness)
   then have "(\<sigma>\<^sub>x |` \<L> x) ++ (\<sigma>' |` \<L> y) = (\<sigma>' |` \<L> x) ++ (\<sigma>' |` \<L> y)"
     by (metis (no_types, lifting) CodeGenAlt.compatible.elims(2) \<open>\<sigma>\<^sub>x ++ \<sigma>' = \<sigma>'\<close> comp map_add_None map_le_def restricted_unchanged)
   then have "(\<sigma>\<^sub>x |` \<L> x) ++ (\<sigma>' |` \<L> y) = (\<sigma>' |` (\<L> x \<union> \<L> y))"
@@ -770,27 +793,27 @@ next
   then show ?case using mt1 mt2 e'
     using match_tree.simps(2) by presburger
 next
-  case (6 c \<Sigma> c\<^sub>m c\<^sub>v \<Sigma>\<^sub>c t t\<^sub>m t\<^sub>v \<Sigma>\<^sub>t f f\<^sub>m f\<^sub>v \<Sigma>\<^sub>f v')
+  case (ConditionalPattern c \<Sigma> c\<^sub>m c\<^sub>v \<Sigma>\<^sub>c t t\<^sub>m t\<^sub>v \<Sigma>\<^sub>t f f\<^sub>m f\<^sub>v \<Sigma>\<^sub>f v')
   then show ?case sorry
 next
-  case (7 vn \<Sigma>)
+  case (ConstantVariableUnseen vn \<Sigma>)
   then show ?case sorry
 next
-  case (8 vn \<Sigma> v')
+  case (ConstantVariableSeen vn \<Sigma> v')
   have "v' \<noteq> vn"
-    using "8.hyps" "8.prems"(3) valid_pattern_preserves_freshness
-    using "8.prems"(1) freshness by force
+    using ConstantVariableSeen valid_pattern_preserves_freshness
+    using freshness by force
   also have "\<sigma>' = \<sigma>(v' \<mapsto> e')"
-    using "8.prems"(3) calculation(1) 
+    using ConstantVariableSeen calculation(1) 
     using eval_match.simps by blast
   ultimately show ?case
-    using "8.prems"(1) eval_match_equality sorry
+    using ConstantVariableSeen eval_match_equality sorry
 next
-  case (9 v' \<Sigma> nid s)
+  case (ParameterPattern v' \<Sigma> nid s)
   then show ?case
     using eval_match_ParameterExpr by fastforce
 next
-  case (10 v' \<Sigma> nid s)
+  case (LeafPattern v' \<Sigma> nid s)
   then show ?case
     using eval_match_LeafExpr by fastforce
 qed
